Almost proved sum.

src/coq/proof_system/imp.v
@@ -1,15 +1,13 @@
 (* Imports *)
 Require Import ZArith String Bool .
 Require Import List.
-Require Import Formula .
 Require Import Model .
-Require Import ProofSystem .
 
 Open Scope Z_scope.
 Import ImpModel.
 
 (* Instantiate Terms with IMP syntax *)
-Module ImpSyntax <: TERM .
+Module ImpSyntax (* <: TERM *) .
   
   (* Arithmetic expressions *)
   Inductive AExp :=
@@ -97,8 +95,9 @@ Eval compute in (eval_bexp (("c", 10)::("b", 5)::nil) (bexp_leq (aexp_id "e") (a
   Inductive KSequence :=
     | kra : Stmt -> KSequence -> KSequence 
     | kdot : KSequence .
+  (*
   Notation "K ~> K'" := (kra K K') (at level 99).
-
+   *)
 
   (* Configuration *)
   Inductive Cfg : Type := cfg : KSequence -> State -> Cfg .
@@ -109,7 +108,32 @@ Eval compute in (eval_bexp (("c", 10)::("b", 5)::nil) (bexp_leq (aexp_id "e") (a
 End ImpSyntax.
 
 
-Module Import F := MLFormula (ImpSyntax) .
+(* Module Import F := MLFormula (ImpSyntax) . *)
+Import ImpSyntax .
+  (* Variables - ??? *)
+  Inductive Var : Set := varF : Z -> Var .
+  (* Matching logic formulas *)
+  Inductive Formula : Type :=
+    | bp : Term -> Formula
+    | T : Formula 
+    | andF : Formula -> Formula -> Formula
+    | orF : Formula -> Formula -> Formula
+    | notF : Formula -> Formula
+    | impliesF : Formula -> Formula -> Formula 
+    | existsF : Var -> Formula -> Formula
+    | symF : SymBool -> Formula 
+  .
+   
+  (* Rules = Reachability Logic formulas *)
+  Inductive Rule : Type := rule : Formula -> Formula -> Rule .
+  Notation "L => R" := (rule L R) (at level 100).
+  
+  (* Reachability rules system *)
+  Definition System := Rule -> Prop .
+
+  (* TODO: move this in its own file ? *)
+  Definition Valid (phi : Formula) := True.
+  
 
 
 (* Semantics *)
@@ -119,6 +143,16 @@ Inductive S : System :=
                    S (rule
                         (andF (bp (cfg (kra (stmtAssign X E) K) Env)) P)
                         (andF (bp (cfg (kra stmtSkip K) Env')) P))
+  (* trick -> get rid of delta *)
+  | stepIfElse : forall St1 St2 Env B K P C,
+                   evalBexp Env B = Some C ->
+                   S (rule
+                        (andF (bp (cfg (kra (stmtIfElse B St1 St2) K) Env)) (symF P))
+                        (orF
+                           (andF (bp (cfg (kra St1 K) Env))
+                                 (symF (symAnd C P)))
+                           (andF (bp (cfg (kra St2 K) Env))
+                                 (symF (symAnd (symNeg C) P)))))
 (*  | stepIfElse1 : forall St1 St2 Env B K P V,
                     evalBexp Env B = Some V -> V = true ->
                     S (andF (bp (cfg (kra (stmtIfElse B St1 St2) K) Env)) P)
@@ -153,47 +187,383 @@ Inductive S : System :=
 
 
 
-Module Import PS := ProofSystem.ProofSystem (ImpSyntax) .
+
+(* Module Import PS := ProofSystem.ProofSystem (ImpSyntax) . *)
+
+  (* TODO: implement the functions below *)
+  Fixpoint delta_S (phi : Formula) (S : System) : Formula := phi .
+  Fixpoint delta_G (phi : Formula) (C : Rule) : Formula := phi .
+  Fixpoint covers (r : Rule) (phi : Formula) := True .
+  Fixpoint derivable (phi : Formula) (S : System) := True .
+
+  Inductive PS : System -> System -> Rule -> Prop :=
+    | ps_ss : forall (S : System) (G : System)
+                     (phi : Formula) (phi' : Formula),
+                derivable phi S -> PS S G (phi => (delta_S phi S))
+    | ps_circ : forall (S : System) (G : System)
+                       (phi : Formula) (phi' : Formula) (phi'' : Formula),
+                  G (phi' => phi'') -> covers (phi' => phi'') phi ->
+                  PS S G (phi => (delta_G phi (phi' => phi'')))
+    | ps_impl : forall (S : System) (G : System)
+                       (phi : Formula) (phi' : Formula),
+            Valid (impliesF phi phi') -> PS S G (phi => phi')
+    | ps_ca : forall (S : System) (G : System)
+                     (phi : Formula) (phi' : Formula) (phi'' : Formula),
+                PS S G (phi' => phi) -> PS S G (phi'' => phi)
+                -> PS S G ((orF phi' phi'') => phi)
+    | ps_trans : forall (S : System) (G : System)
+                        (phi : Formula) (phi' : Formula) (phi'' : Formula),
+                   PS S G (phi => phi'') -> PS S G (phi'' => phi') -> PS S G (phi => phi') .
+
+
+
+
+
+
+
 Open Scope string_scope .
 
 Inductive G : System :=
-  | circularity : forall N S I, 
-                    G (rule (andF
-                               (bp
-                                  (cfg
-                                     (kra (stmtWhile (bexpLeq (aexpId "i") (aexpId "n"))
-                                                     (stmtList (stmtAssign "s" (aexpPlus (aexpId "s") (aexpId "i")))
-                                                               (stmtAssign "i" (aexpPlus (aexpId "i") (aexpSymInt (symZ 1)) ))))
-                                          kdot)
-                                     (("n", N)::("i", I)::("s", S)::nil) ))
-                               (symF (symAnd
-                                        (symLeInt (symZ 0) N)
-                                        (symEqInt S (symDiv (symMult I (symPlus I (symZ 1))) (symZ 2)))
-                                     ))
-                            )
-                            (andF (bp (cfg (kra stmtSkip kdot)
-                                           (("n", N)::("i", (symPlus I (symZ 1)))::("s", (symDiv (symMult (symPlus I (symZ 1)) (symPlus I (symZ 2))) (symZ 2)))::nil))) T)) .
+  | circularity : forall N Sum I, 
+                    G ((andF
+               (bp
+                  (cfg
+                     (kra (stmtWhile (bexpLeq (aexpId "i") (aexpId "n"))
+                                     (stmtList (stmtAssign "s" (aexpPlus (aexpId "s") (aexpId "i")))
+                                               (stmtAssign "i" (aexpPlus (aexpId "i") (aexpSymInt (symZ 1)) ))))
+                          kdot)
+                     (("n", N)::("i", I)::("s", Sum)::nil) ))
+               (symF (symAnd
+                        (symLeInt (symZ 0) N)
+                        (symEqInt Sum (symDiv (symMult I (symPlus I (symZ 1))) (symZ 2)))
+                     ))
+            )
+            =>
+            (andF (bp (cfg (kra stmtSkip kdot)
+                           (("n", N)::("i", (symPlus I (symZ 1)))::("s", (symDiv (symMult (symPlus I (symZ 1)) (symPlus I (symZ 2))) (symZ 2)))::nil))) T)) .
 
-Print System .
-Print F.System.
-Print Rule .
-Print F.Rule .
-Print Formula .
-Print F.Formula .
 
-Lemma sum : PS S G (andF
-                      (bp
-                         (cfg
-                            (kra (stmtWhile (bexpLeq (aexpId "i") (aexpId "n"))
-                                            (stmtList (stmtAssign "s" (aexpPlus (aexpId "s") (aexpId "i")))
-                                                      (stmtAssign "i" (aexpPlus (aexpId "i") (aexpSymInt (symZ 1)) ))))
-                                 kdot)
-                            (("n", N)::("i", I)::("s", S)::nil) ))
-                      (symF (symAnd
-                               (symLeInt (symZ 0) N)
-                               (symEqInt S (symDiv (symMult I (symPlus I (symZ 1))) (symZ 2)))
-                            ))
-                   )
-               (andF (bp (cfg (kra stmtSkip kdot)
-                              (("n", N)::("i", (symPlus I (symZ 1)))::("s", (symDiv (symMult (symPlus I (symZ 1)) (symPlus I (symZ 2))) (symZ 2)))::nil))) T) .
+
+Axiom reduceToSem : forall (S : System) (G : System)
+                           (phi : Formula) (phi' : Formula),
+                      S (phi => phi') -> PS S G (phi => phi') .
+
+(* Take care with this! :-) *)
+Axiom reduceToCirc : forall (S : System) (G : System)
+                           (phi : Formula) (phi' : Formula),
+                      G (phi => phi') -> PS S G (phi => phi') .
+
+
   
+
+
+Lemma sum :
+  forall N I Sum,
+    PS S G ((andF
+               (bp
+                  (cfg
+                     (kra (stmtWhile (bexpLeq (aexpId "i") (aexpId "n"))
+                                     (stmtList (stmtAssign "s" (aexpPlus (aexpId "s") (aexpId "i")))
+                                               (stmtAssign "i" (aexpPlus (aexpId "i") (aexpSymInt (symZ 1)) ))))
+                          kdot)
+                     (("n", N)::("i", I)::("s", Sum)::nil) ))
+               (symF (symAnd
+                        (symLeInt (symZ 0) N)
+                        (symEqInt Sum (symDiv (symMult I (symPlus I (symZ 1))) (symZ 2)))
+                     ))
+            )
+            =>
+            (andF (bp (cfg (kra stmtSkip kdot)
+                           (("n", N)::("i", (symPlus I (symZ 1)))::("s", (symDiv (symMult (symPlus I (symZ 1)) (symPlus I (symZ 2))) (symZ 2)))::nil))) T)) .
+Proof.
+  intros.
+
+  apply ps_trans with
+  (phi'' :=
+    (andF
+        (bp
+           (cfg
+              (kra (stmtIfElse (bexpLeq (aexpId "i") (aexpId "n"))
+                          (stmtList
+                          (stmtList
+                             (stmtAssign "s" (aexpPlus (aexpId "s") (aexpId "i")))
+                             (stmtAssign "i"
+                                         (aexpPlus (aexpId "i") (aexpSymInt (symZ 1)))))
+                          (stmtWhile (bexpLeq (aexpId "i") (aexpId "n"))
+                                     (stmtList
+                                        (stmtAssign "s" (aexpPlus (aexpId "s") (aexpId "i")))
+                                        (stmtAssign "i"
+                                                    (aexpPlus (aexpId "i") (aexpSymInt (symZ 1))))))) stmtSkip)
+                   kdot) (("n", N) :: ("i", I) :: ("s", Sum) :: nil)))
+      (symF
+         (symAnd (symLeInt (symZ 0) N)
+                 (symEqInt Sum
+                           (symDiv (symMult I (symPlus I (symZ 1))) (symZ 2))))))
+  ).
+
+
+  - apply reduceToSem.
+    apply stepWhile.
+  - apply ps_trans with
+    (phi'' :=
+       (orF
+          (andF
+             (bp
+                (cfg
+                   (kra 
+                      (stmtList
+                         (stmtAssign "s" (aexpPlus (aexpId "s") (aexpId "i")))
+                         (stmtList
+                            (stmtAssign "i" (aexpPlus (aexpId "i") (aexpSymInt (symZ 1))))
+                            (stmtWhile (bexpLeq (aexpId "i") (aexpId "n"))
+                                       (stmtList
+                                          (stmtAssign "s" (aexpPlus (aexpId "s") (aexpId "i")))
+                                          (stmtAssign "i" (aexpPlus (aexpId "i") (aexpSymInt (symZ 1))))))))
+                   kdot)
+                   (("n", N) :: ("i", I) :: ("s", Sum) :: nil)))
+             (symF
+                (symAnd (symLeInt I N)
+                        (symAnd (symLeInt (symZ 0) N)
+                                (symEqInt Sum (symDiv (symMult I (symPlus I (symZ 1))) (symZ 2)))))))
+          (andF
+             (bp
+                (cfg
+                   (kra stmtSkip kdot)
+                   (("n", N) :: ("i", I) :: ("s", Sum) :: nil)))
+             (symF
+                (symAnd (symNeg (symLeInt I N))
+                        (symAnd (symLeInt (symZ 0) N)
+                                (symEqInt Sum (symDiv (symMult I (symPlus I (symZ 1))) (symZ 2)))))))
+          
+       )).
+    +
+      apply ps_trans with
+      (phi'' := andF
+        (bp
+           (cfg
+              (kra
+                 (stmtIfElse (bexpLeq (aexpId "i") (aexpId "n"))
+                             (stmtList
+                                (stmtAssign "s" (aexpPlus (aexpId "s") (aexpId "i")))
+                                (stmtList
+                                   (stmtAssign "i" (aexpPlus (aexpId "i") (aexpSymInt (symZ 1))))
+                                   (stmtWhile (bexpLeq (aexpId "i") (aexpId "n"))
+                                              (stmtList
+                                                 (stmtAssign "s" (aexpPlus (aexpId "s") (aexpId "i")))
+                                                 (stmtAssign "i" (aexpPlus (aexpId "i") (aexpSymInt (symZ 1)))))))
+                                )
+                    stmtSkip) kdot)
+              (("n", N) :: ("i", I) :: ("s", Sum) :: nil)))
+        (symF
+           (symAnd (symLeInt (symZ 0) N)
+              (symEqInt Sum
+                        (symDiv (symMult I (symPlus I (symZ 1))) (symZ 2)))))
+        ).
+
+      apply ps_impl.
+      unfold Valid. trivial.
+
+      apply reduceToSem.
+      apply stepIfElse.
+      simpl. auto. 
+
+    + apply ps_ca.
+      * apply ps_trans with
+        (phi'' := (
+                   andF
+                     (bp
+                        (cfg
+                           (kra
+                              (stmtAssign "s" (aexpPlus (aexpId "s") (aexpId "i")))
+                              (kra
+                                 (stmtList
+                                    (stmtAssign "i"
+                                                (aexpPlus (aexpId "i") (aexpSymInt (symZ 1))))
+                                    (stmtWhile (bexpLeq (aexpId "i") (aexpId "n"))
+                                               (stmtList
+                                                  (stmtAssign "s" (aexpPlus (aexpId "s") (aexpId "i")))
+                                                  (stmtAssign "i" (aexpPlus (aexpId "i") (aexpSymInt (symZ 1)))))))
+                                 kdot))
+                           (("n", N) :: ("i", I) :: ("s", Sum) :: nil)))
+                     (symF
+                        (symAnd (symLeInt I N)
+                                (symAnd (symLeInt (symZ 0) N)
+                                        (symEqInt Sum
+                                                  (symDiv (symMult I (symPlus I (symZ 1))) (symZ 2))))))
+                 )).
+        
+        apply reduceToSem.
+        apply stepList.
+
+        apply ps_trans with
+        (phi'' :=
+           (andF
+              (bp
+                 (cfg
+                    (kra stmtSkip
+                         (kra
+                            (stmtList
+                               (stmtAssign "i"
+                                           (aexpPlus (aexpId "i") (aexpSymInt (symZ 1))))
+                               (stmtWhile (bexpLeq (aexpId "i") (aexpId "n"))
+                                          (stmtList
+                                             (stmtAssign "s" (aexpPlus (aexpId "s") (aexpId "i")))
+                                             (stmtAssign "i" (aexpPlus (aexpId "i") (aexpSymInt (symZ 1)))))))
+                            kdot)) (("n", N) :: ("i", I) :: ("s", (symPlus Sum I)) :: nil)))
+              (symF
+                 (symAnd (symLeInt I N)
+                         (symAnd (symLeInt (symZ 0) N)
+                                 (symEqInt Sum
+                                           (symDiv (symMult I (symPlus I (symZ 1))) (symZ 2))))))
+           )).
+
+        apply reduceToSem.
+
+        (*  evalAexp Env E = Some V -> update X V Env = Some Env'  *)
+(*        Eval compute in  evalAexp (("n", N) :: ("i", I) :: ("s", Sum) :: nil)
+                                   (aexpPlus (aexpId "s") (aexpId "i")).
+*)        
+        apply stepAssign with (V := (symPlus Sum I)) .
+        simpl. trivial.
+        simpl. trivial.
+        
+
+        apply ps_trans with
+        (phi'' :=
+           (andF
+              (bp
+                 (cfg
+                         (kra
+                            (stmtList
+                               (stmtAssign "i"
+                                           (aexpPlus (aexpId "i") (aexpSymInt (symZ 1))))
+                               (stmtWhile (bexpLeq (aexpId "i") (aexpId "n"))
+                                          (stmtList
+                                             (stmtAssign "s"
+                                (aexpPlus (aexpId "s") (aexpId "i")))
+                                             (stmtAssign "i"
+                                                         (aexpPlus (aexpId "i") (aexpSymInt (symZ 1)))))))
+                            kdot)
+                    (("n", N) :: ("i", I) :: ("s", symPlus Sum I) :: nil)))
+              (symF
+                 (symAnd (symLeInt I N)
+                         (symAnd (symLeInt (symZ 0) N)
+                                 (symEqInt Sum
+                                           (symDiv (symMult I (symPlus I (symZ 1))) (symZ 2))))))
+           )
+        ).
+
+        apply reduceToSem.
+        apply stepSkip.
+
+
+
+        apply ps_trans with
+        (phi'' :=
+           (andF
+        (bp
+           (cfg
+              (kra
+                 (stmtAssign "i"
+                       (aexpPlus (aexpId "i") (aexpSymInt (symZ 1))))
+                 (kra
+                    
+                    (stmtWhile (bexpLeq (aexpId "i") (aexpId "n"))
+                       (stmtList
+                          (stmtAssign "s" (aexpPlus (aexpId "s") (aexpId "i")))
+                          (stmtAssign "i" (aexpPlus (aexpId "i") (aexpSymInt (symZ 1))))))
+                 kdot)) (("n", N) :: ("i", I) :: ("s", symPlus Sum I) :: nil)))
+        (symF
+           (symAnd (symLeInt I N)
+              (symAnd (symLeInt (symZ 0) N)
+                 (symEqInt Sum
+                    (symDiv (symMult I (symPlus I (symZ 1))) (symZ 2))))))
+        )).
+
+
+        apply reduceToSem.
+        apply stepList.
+
+
+        apply ps_trans with
+        (phi'' :=
+           (andF
+              (bp
+                 (cfg
+                    (kra
+                       stmtSkip
+                       (kra
+                          (stmtWhile (bexpLeq (aexpId "i") (aexpId "n"))
+                                     (stmtList
+                                        (stmtAssign "s"
+                                                    (aexpPlus (aexpId "s") (aexpId "i")))
+                                        (stmtAssign "i"
+                                                    (aexpPlus (aexpId "i") (aexpSymInt (symZ 1))))))
+                          kdot))
+                    (("n", N) :: ("i", symPlus I (symZ 1)) :: ("s", symPlus Sum I) :: nil)))
+              (symF
+                 (symAnd (symLeInt I N)
+                         (symAnd (symLeInt (symZ 0) N)
+                                 (symEqInt Sum
+                                           (symDiv (symMult I (symPlus I (symZ 1))) (symZ 2)))))))
+        ).
+
+        apply reduceToSem.
+        apply stepAssign with (V := symPlus I (symZ 1)).
+        simpl. trivial.
+        simpl. trivial.
+
+        apply ps_trans with
+        (phi'' :=
+           (andF
+              (bp
+                 (cfg
+                         (kra
+                            (stmtWhile (bexpLeq (aexpId "i") (aexpId "n"))
+                                       (stmtList
+                                          (stmtAssign "s" (aexpPlus (aexpId "s") (aexpId "i")))
+                                          (stmtAssign "i" (aexpPlus (aexpId "i") (aexpSymInt (symZ 1))))))
+                            kdot)
+                    (("n", N)
+                       :: ("i", symPlus I (symZ 1)) :: ("s", symPlus Sum I) :: nil)))
+              (symF
+                 (symAnd (symLeInt I N)
+                         (symAnd (symLeInt (symZ 0) N)
+                                 (symEqInt Sum
+                                           (symDiv (symMult I (symPlus I (symZ 1))) (symZ 2)))))))
+        ).
+
+        apply reduceToSem.
+        apply stepSkip.
+
+
+        (* prepare for circularity *)
+        apply ps_trans with
+        (phi'' :=
+           (andF
+               (bp
+                  (cfg
+                     (kra (stmtWhile (bexpLeq (aexpId "i") (aexpId "n"))
+                                     (stmtList (stmtAssign "s" (aexpPlus (aexpId "s") (aexpId "i")))
+                                               (stmtAssign "i" (aexpPlus (aexpId "i") (aexpSymInt (symZ 1)) ))))
+                          kdot)
+                     (("n", N)::("i", I)::("s", Sum)::nil) ))
+               (symF (symAnd
+                        (symLeInt (symZ 0) N)
+                        (symEqInt Sum (symDiv (symMult I (symPlus I (symZ 1))) (symZ 2)))
+                     ))
+           )
+        ).
+
+        apply ps_impl.
+        unfold Valid. trivial.
+
+
+        (* circularity -> apply ps_circ. *)
+        apply reduceToCirc.
+        apply circularity.
+
+      * apply ps_impl.
+        unfold Valid. trivial.
+Qed.
+
